Leslie_LTS/Examples.lean
@@ -3,6 +3,7 @@ import Leslie_LTS.Examples.BCA
 import Leslie_LTS.Examples.BCA_Simulation
 import Leslie_LTS.Examples.BrachaBRB
 import Leslie_LTS.Examples.BRB_Simulation
+import Leslie_LTS.Examples.BRB_Liveness
 import Leslie_LTS.Examples.CorruptionInvariants
 import Leslie_LTS.Examples.DoubleBCA
 import Leslie_LTS.Examples.DoubleBCA_Simulation
